src/checker/Pulse.Extract.Main.fst
@@ -111,7 +111,7 @@ let is_internal_binder (b:binder) : T.Tac bool =
   s = "_tbind_c" ||
   s = "_if_br" ||
   s = "_br" ||
-  s = "_"
+  s = "__"
 
 let is_return (e:st_term) : option term =
   match e.term with
